examples/quicksort/Partition.v
@@ -23,17 +23,17 @@ Implicit Arguments On.
  * that all elements of a segment [g,d] are <= (resp. >=) than a given value
  *)
 
-Inductive array_le [N:Z; t:(array N Z) ; g,d,v:Z] : Prop
+Inductive array_le [t:(array Z) ; g,d,v:Z] : Prop
   := array_le_cons :
      ((i:Z) `g <= i <= d` -> (Zle #t[i] v))
   -> (array_le t g d v).
 
-Inductive array_ge [N:Z; t:(array N Z) ; g,d,v:Z] : Prop
+Inductive array_ge [t:(array Z) ; g,d,v:Z] : Prop
   := array_ge_cons :
      ((i:Z) `g <= i <= d` -> (Zle v #t[i]))
   -> (array_ge t g d v).
 
-Inductive partition_p [N:Z; t:(array N Z) ; g,d,p:Z] : Prop
+Inductive partition_p [t:(array Z) ; g,d,p:Z] : Prop
   := piv : `g <= p` -> `p <= d`
          -> (array_le t g `p-1` #t[p])
          -> (array_ge t `p+1` d #t[p])
@@ -43,22 +43,22 @@ Inductive partition_p [N:Z; t:(array N Z) ; g,d,p:Z] : Prop
 (* Lemmas about array_le *)
 
 Lemma array_le_empty :
-  (N:Z)(t:(array N Z))(g,d,v:Z)
+  (t:(array Z))(g,d,v:Z)
     `d < g`
     -> (array_le t g d v).
 Proof.
-Intros N t g d v H.
+Intros t g d v H.
 Constructor. Intros.
 Absurd `g<=d`; Omega.
 Save.
 
 Lemma array_le_right_extension :
-  (N:Z)(t:(array N Z))(g,d,v:Z)
+  (t:(array Z))(g,d,v:Z)
     (array_le t g d v)
     -> (Zle #t[`d+1`] v)
       -> (array_le t g `d+1` v).
 Proof.
-Intros N t g d v H_le Hv.
+Intros t g d v H_le Hv.
 Elim H_le; Intros.
 Constructor. Intros.
 Elim (Z_eq_dec i `d+1`); Intro.
@@ -67,40 +67,40 @@ Apply H; Omega.
 Save.
 
 Lemma array_le_exchange :
-  (N:Z)(t,t':(array N Z))(g,d,v:Z)(x,y:Z)
-    `0 <= g` -> `d < N`
+  (t,t':(array Z))(g,d,v:Z)(x,y:Z)
+    `0 <= g` -> `d < (array_length t)`
     -> (array_le t g d v)
     -> `d < x <= y`
       -> (exchange t t' x y)
         -> (array_le t' g d v).
 Proof.
-Intros N t t' g d v x y Hg Hd Hle Hxy Hex.
+Intros t t' g d v x y Hg Hd Hle Hxy Hex.
 Elim Hle; Intros. 
 Elim Hex; Intros.
 Constructor. Intros.
-Rewrite <- H4; Try Omega.
+Rewrite <- H5; Try Omega.
 Apply H; Assumption.
 Save.
 
 (* Lemmas about array_ge *)
 
 Lemma array_ge_empty :
-  (N:Z)(t:(array N Z))(g,d,v:Z)
+  (t:(array Z))(g,d,v:Z)
     `d < g`
     -> (array_ge t g d v).
 Proof.
-Intros N t g d v H.
+Intros t g d v H.
 Constructor. Intros.
 Absurd `g<=d`; Omega.
 Save.
 
 Lemma array_ge_left_extension :
-  (N:Z)(t:(array N Z))(g,d,v:Z)
+  (t:(array Z))(g,d,v:Z)
     (array_ge t g d v)
     -> (Zle v #t[`g-1`])
       -> (array_ge t `g-1` d v).
 Proof.
-Intros N t g d v H_ge Hv.
+Intros t g d v H_ge Hv.
 Elim H_ge; Intros.
 Constructor. Intros.
 Elim (Z_eq_dec i `g-1`); Intro.
@@ -109,18 +109,18 @@ Apply H; Omega.
 Save.
 
 Lemma array_ge_exchange :
-  (N:Z)(t,t':(array N Z))(g,d,v:Z)(x,y:Z)
-    `0 <= g` -> `d < N`
+  (t,t':(array Z))(g,d,v:Z)(x,y:Z)
+    `0 <= g` -> `d < (array_length t)`
     -> (array_ge t g d v)
     -> `x <= y < g`
       -> (exchange t t' x y)
         -> (array_ge t' g d v).
 Proof.
-Intros N t t' g d v x y Hg Hd Hge Hxy Hex.
+Intros t t' g d v x y Hg Hd Hge Hxy Hex.
 Elim Hge; Intros. 
 Elim Hex; Intros.
 Constructor. Intros.
-Rewrite <- H4; Try Omega.
+Rewrite <- H5; Try Omega.
 Apply H; Assumption.
 Save.
 
@@ -128,20 +128,20 @@ Save.
 (* Lemmas about partition_p and sub_permut *)
 
 Lemma partition_p_permut_left :
-  (N:Z)(t,t':(array N Z))(g,d,p:Z)
-  `0 <= g` -> `g < d` -> `d < N` -> `g <= p <= d`
+  (t,t':(array Z))(g,d,p:Z)
+  `0 <= g` -> `g < d` -> `d < (array_length t)` -> `g <= p <= d`
   -> (partition_p t g d p)
   -> (sub_permut g (Zpred p) t t')
   -> (partition_p t' g d p).
 Proof.
-Intros N t t' g d p hyp1 hyp2 hyp3 hyp4 piv_t perm.
+Intros t t' g d p hyp1 hyp2 hyp3 hyp4 piv_t perm.
 Elim piv_t; Intros.
-Cut `(Zpred p)<N` ; [ Intro | Unfold Zpred; Omega ].
-Generalize (sub_permut_function hyp1 H3 perm). Intro.
+Cut `(Zpred p)<(array_length t)` ; [ Intro | Unfold Zpred; Omega ].
+Generalize (sub_permut_function perm hyp1 H3). Intro.
 Constructor; Try Assumption.
 (* array_le *)
 Constructor. Intros.
-Rewrite <- (sub_permut_eq perm 8!p).
+Rewrite <- (sub_permut_eq perm 7!p).
 Elim H1; Intros.
 Elim (H4 i); Try (Unfold Zpred; Omega). Intros.
 Elim H8; Intros.
@@ -150,8 +150,8 @@ Apply H6; Unfold Zpred in H10; Omega.
 Unfold Zpred; Omega.
 (* array_ge *)
 Constructor. Intros.
-Rewrite <- (sub_permut_eq perm 8!p).
-Rewrite <- (sub_permut_eq perm 8!i).
+Rewrite <- (sub_permut_eq perm 7!p).
+Rewrite <- (sub_permut_eq perm 7!i).
 Elim H2; Intros.
 Apply H6; Omega.
 Unfold Zpred; Omega.
@@ -160,28 +160,28 @@ Save.
 
 
 Lemma partition_p_permut_right :
-  (N:Z)(t,t':(array N Z))(g,d,p:Z)
-  `0 <= g` -> `g < d` -> `d < N` -> `g <= p <= d`
+  (t,t':(array Z))(g,d,p:Z)
+  `0 <= g` -> `g < d` -> `d < (array_length t)` -> `g <= p <= d`
   -> (partition_p t g d p)
   -> (sub_permut (Zs p) d t t')
   -> (partition_p t' g d p).
 Proof.
-Intros N t t' g d p hyp1 hyp2 hyp3 hyp4 piv_t perm.
+Intros t t' g d p hyp1 hyp2 hyp3 hyp4 piv_t perm.
 Elim piv_t; Intros.
 Cut `0<=(Zs p)` ; [ Intro | Unfold Zpred; Omega ].
-Generalize (sub_permut_function H3 hyp3 perm). Intro.
+Generalize (sub_permut_function perm H3 hyp3). Intro.
 Constructor; Try Assumption.
 (* array_le *)
 Constructor. Intros.
-Rewrite <- (sub_permut_eq perm 8!p).
-Rewrite <- (sub_permut_eq perm 8!i).
+Rewrite <- (sub_permut_eq perm 7!p).
+Rewrite <- (sub_permut_eq perm 7!i).
 Elim H1; Intros.
 Apply H6; Omega.
 Unfold Zs; Omega.
 Unfold Zs; Omega.
 (* array_ge *)
 Constructor. Intros.
-Rewrite <- (sub_permut_eq perm 8!p).
+Rewrite <- (sub_permut_eq perm 7!p).
 Elim H2; Intros.
 Elim (H4 i); Try (Unfold Zs; Omega). Intros.
 Elim H8; Intros.
